s->v chapter 7

chapter07/demo/demo01.dfy
@@ -1,15 +1,15 @@
-datatype MapState = MapState(m:map<int, string>)
+datatype MapVariables = MapVariables(m:map<int, string>)
 
-predicate MapInsert(s:MapState, s':MapState, k:int, v:string) {
-  s'.m == s.m[k := v]
+predicate MapInsert(v:MapVariables, v':MapVariables, k:int, value:string) {
+  v'.m == v.m[k := value]
 }
 
-predicate MapNext(s:MapState, s':MapState) {
-  exists k, v :: MapInsert(s, s', k, v)
+predicate MapNext(v:MapVariables, v':MapVariables) {
+  exists k, value :: MapInsert(v, v', k, value)
 }
 
 
-datatype Slot = Empty | Used(k:int, v:string)
+datatype Slot = Empty | Used(k:int, value:string)
 datatype HashTblState = HashTblState(tbl:seq<Slot>)
 
 datatype OptionIndex = None | Some(idx:nat)
@@ -22,20 +22,20 @@ function Probe(tbl:seq<Slot>, k: int) : (oi:OptionIndex)
   if |tbl|>0 && tbl[0].Empty? then Some(0) else None
 }
 
-predicate HTInsert(s:HashTblState, s':HashTblState, k:int, v:string) {
-  var oi := Probe(s.tbl, k);
+predicate HTInsert(v:HashTblState, v':HashTblState, k:int, value:string) {
+  var oi := Probe(v.tbl, k);
   && oi.Some?
-  && s'.tbl == s.tbl[oi.idx := Used(k, v)]
+  && v'.tbl == v.tbl[oi.idx := Used(k, value)]
 }
 
-predicate HTNext(s:HashTblState, s':HashTblState) {
-  exists k, v :: HTInsert(s, s', k, v)
+predicate HTNext(v:HashTblState, v':HashTblState) {
+  exists k, value :: HTInsert(v, v', k, value)
 }
 
 function InterpRecurse(tbl:seq<Slot>) : (m:map<int, string>)
   ensures m.Keys == set i | 0<=i<|tbl| && tbl[i].Used? :: tbl[i].k
   ensures forall k | k in m ::
-    (exists i :: 0<=i<|tbl| && tbl[i].Used? && m[tbl[i].k]==tbl[i].v)
+    (exists i :: 0<=i<|tbl| && tbl[i].Used? && m[tbl[i].k]==tbl[i].value)
 {
   if |tbl| == 0
   then map[]
@@ -44,30 +44,30 @@ function InterpRecurse(tbl:seq<Slot>) : (m:map<int, string>)
     var last := tbl[|tbl|-1];
     match last
       case Empty => prefix
-      case Used(k, v) => prefix[k := v]
+      case Used(k, value) => prefix[k := value]
 }
 
-function Interp(ls:HashTblState) : (hs:MapState)
+function Interp(ls:HashTblState) : (hs:MapVariables)
   ensures hs.m.Keys == set i | 0<=i<|ls.tbl| && ls.tbl[i].Used? :: ls.tbl[i].k
   ensures forall k | k in hs.m ::
     (exists i ::
       && 0<=i<|ls.tbl|
       && ls.tbl[i].Used?
-      && hs.m[ls.tbl[i].k]==ls.tbl[i].v)
+      && hs.m[ls.tbl[i].k]==ls.tbl[i].value)
 {
-  MapState(InterpRecurse(ls.tbl))
+  MapVariables(InterpRecurse(ls.tbl))
 }
 
 // Here's a lemma I should prove after I define Inits; without Inits
 // we don't have state-machine-defined behaviors!
-//lemma RefinementInit(ls:HashTblState, hs:MapState)
+//lemma RefinementInit(ls:HashTblState, hs:MapVariables)
 //  requires HTInit(ls)
 //  requires MapInit(hs)
 //  ensures Interp(ls) == hs
 //{
 //}
 
-lemma RefinementInductive(ls:HashTblState, ls':HashTblState, hs:MapState, hs':MapState)
+lemma RefinementInductive(ls:HashTblState, ls':HashTblState, hs:MapVariables, hs':MapVariables)
   requires HTNext(ls, ls')
   requires MapNext(hs, hs')
   // NB you might also require HTInv(ls)
